replaced the automatic tactic by a theorem

Examples_automation.v
@@ -3,79 +3,77 @@ From Views Require Import Lemmas.
 From Views Require Import BoundedInt.
 From Views Require Import ViewFunctions.
 From Views Require Import ViewsProof.
-From Ltac2 Require Import Ltac2.
-From Views Require Import Tactic.
+(* From Ltac2 Require Import Ltac2.
+From Views Require Import Tactic. *)
 Require Import PeanoNat.
 
 (** Proofs that are in `ViewsProof.v` using the automated tactics from `Tactic.v`.
 Does not contain the proof of `map` preserving injectivity as it is not easily automatable by
 following a similar pattern as the others *)
 
-Theorem reverse_preserves_injectivity_auto_proof : forall T n, preserve_Injectivity reverse (A := (n::T)).
+Theorem reverse_preserves_injectivity_auto_proof : forall T n, preserve_Injectivity (view reverse) (A := (n::T)).
 Proof.
   intros T n.
-  set (function := fun (x : Tuple (n::T)) => match x with | (i,tx) => (idx n (n - 1 - to_nat i) reverseProof,tx) end).
-  assert (H':forall (x y : Idx n), n - 1 - to_nat x = n - 1 - to_nat y -> x = y). {
-    (* assertion : the reordering function used by reverse is injective *)
-    intros.
-    apply sub_injective in H.
-    apply to_nat_injective in H. subst. reflexivity.
-    destruct n. destruct x as [nx Hx]. inversion Hx. simpl. rewrite Nat.sub_0_r. apply le_S_n. apply BoundedInt.
-    destruct n. destruct y as [ny Hy]. inversion Hy. simpl. rewrite Nat.sub_0_r. apply le_S_n. apply BoundedInt.
-  }
-  reordering_autoProof ('function) (@function) 0.
-  apply H' in H0; subst; reflexivity.
-  apply H' in H2; subst; reflexivity.
+  apply injective_functions_preserve_injectivity.
+  intros. destruct x as [x tx], y as [y ty].
+  inversion H.
+  apply sub_injective in H1.
+  apply to_nat_injective in H1. subst. reflexivity.
+  destruct n. destruct x as [nx Hx]. inversion Hx. simpl. rewrite Nat.sub_0_r. apply le_S_n. apply BoundedInt.
+  destruct n. destruct y as [ny Hy]. inversion Hy. simpl. rewrite Nat.sub_0_r. apply le_S_n. apply BoundedInt.
 Qed.
 
-Theorem take_left_preserves_injectivity_auto_proof : forall T n b, preserve_Injectivity (take_left b) (A := ((b+n)::T)).
+Theorem take_left_preserves_injectivity_auto_proof : forall T n b, preserve_Injectivity (view (take_left b)) (A := ((b+n)::T)).
 Proof.
   intros T n b.
-  set (function := fun (x : Tuple (b::T)) => match x with | (i,tx) => (idx (b+n) (to_nat i) takeleftProof,tx) end).
-  reordering_autoProof ('function) (@function) 0.
-  - apply to_nat_injective in H0. subst. reflexivity.
-  - apply to_nat_injective in H2. subst. reflexivity.
+  apply injective_functions_preserve_injectivity.
+  intros. destruct x as [x tx], y as [y ty].
+  inversion H.
+  apply to_nat_injective in H1.
+  subst; reflexivity.
 Qed.
 
-Theorem select_range_preserves_injectivity_auto_proof : forall T n a b, preserve_Injectivity (select_range a b) (A := ((b+n)::T)).
-Proof.
-  intros T n a b.
-  set (function := fun (x : Tuple ((b-a)::T)) => match x with | (i,tx) => (idx (b+n) (a + to_nat i) selectrangeProof,tx) end).
-  reordering_autoProof ('function) (@function) 0.
-  - apply add_injective in H0. apply to_nat_injective in H0. subst. reflexivity.
-  - apply add_injective in H2. apply to_nat_injective in H2. subst. reflexivity.
-Qed.
-
-Theorem take_right_preserves_injectivity_auto_proof : forall T n a, preserve_Injectivity (take_right a) (A := ((a+n)::T)).
+Theorem take_right_preserves_injectivity_auto_proof : forall T n a, preserve_Injectivity (view (take_right a)) (A := ((a+n)::T)).
 Proof.
   intros T n a.
-  set (function := fun (x : Tuple (n::T)) => match x with | (i,tx) => (idx (a+n) (a + to_nat i) takerightProof,tx) end).
-  reordering_autoProof ('function) (@function) 0.
-  - apply add_injective in H0. apply to_nat_injective in H0. subst. reflexivity.
-  - apply add_injective in H2. apply to_nat_injective in H2. subst. reflexivity.
+  apply injective_functions_preserve_injectivity.
+  intros. destruct x as [x tx], y as [y ty].
+  inversion H.
+  apply add_injective in H1. apply to_nat_injective in H1.
+  subst; reflexivity.
 Qed.
 
-Theorem transpose_preserves_injectivity_auto_proof : forall T n m, preserve_Injectivity transpose (A := (m::n::T)).
+Theorem select_range_preserves_injectivity_auto_proof : forall T n a b, preserve_Injectivity (view (select_range a b)) (A := ((b+n)::T)).
 Proof.
-  intros T n m.
-  set (function := fun (x : Tuple (n::m::T)) => match x with | (i,(j,tx)) => (j,(i,tx)) end).
-  reordering_autoProof ('function) (@function) 1;
-  reflexivity.
+  intros T n a b.
+  apply injective_functions_preserve_injectivity.
+  intros. destruct x as [x tx], y as [y ty].
+  inversion H.
+  apply add_injective in H1. apply to_nat_injective in H1.
+  subst; reflexivity.
 Qed.
 
-Theorem group_preserves_injectivity_auto_proof : forall T n m, preserve_Injectivity (group m) (A := (m*n::T)).
+Theorem transpose_preserves_injectivity_auto_proof : forall T n m, preserve_Injectivity (view transpose) (A := (m::n::T)).
+Proof.
+  intros T n a b.
+  apply injective_functions_preserve_injectivity.
+  unfold transpose.
+  intros. destruct x as [xi tx], tx as [xj tx], y as [yi ty], ty as [yj ty].
+  inversion H;subst;reflexivity.
+Qed.
+
+Theorem group_preserves_injectivity_auto_proof : forall T n m, preserve_Injectivity (view (group m)) (A := (m*n::T)).
 Proof.
   intros T n m.
-  set (function := fun (x : Tuple (n::m::T)) => match x with | (i,(j,tx)) => (idx (m*n) (to_nat j + m*(to_nat i)) groupProof,tx) end).
-  assert (H':forall (x1 y1 : Idx m) (x2 y2 : Idx n), to_nat x1 + m * to_nat x2 = to_nat y1 + m * to_nat y2 -> (x1,x2) = (y1,y2)). {
-    (* assertion : the reordering function used by reverse is injective *)
-    intros.
-    apply projection_injective in H. inversion H. apply to_nat_injective in H1. apply to_nat_injective in H2. subst. reflexivity.
-    apply BoundedInt. apply BoundedInt.
-  }
-  reordering_autoProof ('function) (@function) 1.
-  apply H' in H0; inversion H0; subst; reflexivity.
-  apply H' in H2; inversion H2; subst; reflexivity.
+  apply injective_functions_preserve_injectivity.
+  intros. destruct x as [xi tx], tx as [xj tx], y as [yi ty], ty as [yj ty].
+  inversion H.
+  apply projection_injective in H1.
+  inversion H1.
+  apply to_nat_injective in H3.
+  apply to_nat_injective in H4.
+  subst;reflexivity.
+  apply BoundedInt. apply BoundedInt.
 Qed.
 
 Fixpoint eqb (m : nat) (n : nat) :=
@@ -103,23 +101,22 @@ Proof.
   - simpl. apply IHn.
 Qed.
 
-Definition swap {T : List nat} {n : nat} (i : Idx n) (j : Idx n) (v : ViewArray [[T;n]]) : ViewArray [[T;n]] :=
-  fun i' => if (eqb (to_nat i') (to_nat i)) then v j else if (eqb (to_nat i') (to_nat j)) then v i else v i'.
+Definition swap {T : List nat} {n : nat} (i : Idx n) (j : Idx n) : Tuple (n::T) -> Tuple (n::T) :=
+  fun x => match x with | (i',x) => (if (eqb (to_nat i') (to_nat i)) then j else if (eqb (to_nat i') (to_nat j)) then i else i',x) end.
 
 Theorem test_auto_swap :
-  forall T n (i j : Idx n), preserve_Injectivity (swap i j) (A := (n::T)).
+  forall T n (i j : Idx n), preserve_Injectivity (view (swap i j)) (A := (n::T)).
 Proof.
   intros T n i j.
-  set (function := fun (x : Tuple (n::T)) =>
-                   match x with | (i',tx) =>
-                   (if (eqb (to_nat i') (to_nat i)) then j else if (eqb (to_nat i') (to_nat j)) then i else i',tx) end).
-  auto_destruct 0;
+  apply injective_functions_preserve_injectivity.
+  unfold swap.
+  intros.
+  destruct x as [i0 tx],y as [i1 ty].
   (* destruct equalities *)
   destruct (eqb (to_nat i0) (to_nat i)) eqn:Ex;
   destruct (eqb (to_nat i0) (to_nat j)) eqn:Ex';
   destruct (eqb (to_nat i1) (to_nat i)) eqn:Ey;
   destruct (eqb (to_nat i1) (to_nat j)) eqn:Ey';
-  unfold swap in *; simpl in Hypothesis1;
   (* replace eqb by actual equalities *)
   try (rewrite Ex in Hypothesis1);
   try (apply eqb_impl_eq in Ex; apply to_nat_injective in Ex);
@@ -129,26 +126,11 @@ Proof.
   try (apply eqb_impl_eq in Ey; apply to_nat_injective in Ey);
   try (rewrite Ey' in Hypothesis1);
   try (apply eqb_impl_eq in Ey'; apply to_nat_injective in Ey');
-  auto_apply(); try reflexivity. (* solve 24 of the 32 cases *)
-  (* manually handling the absurd cases *)
+  inversion H; subst; try reflexivity.
+  (* handling the absurd cases *)
   rewrite eqb_n_n in Ey';inversion Ey'.
   rewrite eqb_n_n in Ey;inversion Ey.
   rewrite eqb_n_n in Ex';inversion Ex'.
   rewrite eqb_n_n in Ex;inversion Ex.
-  rewrite eqb_n_n in Ey';inversion Ey'.
-  rewrite eqb_n_n in Ey;inversion Ey.
-  rewrite eqb_n_n in Ex';inversion Ex'.
-  rewrite eqb_n_n in Ex;inversion Ex.
-Qed.
-
-Theorem test_auto_permutation :
-  forall T n (f : Idx n -> Idx n),
-  (forall x y, f x = f y -> x = y) -> preserve_Injectivity (fun v i => v (f i)) (A := n::T)  (B := (n::T)).
-Proof.
-  intros T n f Hf.
-  set (function := fun (x : Tuple (n::T)) => match x with | (i,ti) => (f i,ti) end).
-  reordering_autoProof ('function) (@function) 0.
-  apply Hf in H0. subst. reflexivity.
-  apply Hf in H2. subst. reflexivity.
 Qed.
 
