ViewsProof.v
@@ -6,17 +6,27 @@ From Views Require Import ViewsLemmas.
 Require Import PeanoNat.
 
 
+
+Definition view {A : List nat} {B : List nat} (f : Tuple B -> Tuple A) : (CurryViewArray A -> CurryViewArray B) :=
+  fun v x => v (f x)
+.
+
+Definition currying {A : List nat} : ViewArray A -> CurryViewArray A :=
+  fun v x => curry_totalApp v x
+.
+
 (*
 preserve_Injectivity f <-> (fun (g : C -> ViewArray A) x y -> f (g x) y) preserves injectivity of g
 *)
-Definition preserve_Injectivity {A : List nat} {B : List nat} (f : ViewArray A -> ViewArray B) :=
+Definition preserve_Injectivity {A : List nat} {B : List nat} (f : CurryViewArray A -> CurryViewArray B) :=
   forall (C : List nat) (v : ViewArray (C++A)),
   Injective v ->
   (forall (i j : Tuple C) (x y : Tuple B),
-  curry_totalApp (f (curry_partialApp v i)) x = curry_totalApp (f (curry_partialApp v j)) y -> (i,x) = (j,y)).
+  (f (currying (curry_partialApp v i))) x = (f (currying (curry_partialApp v j))) y -> (i,x) = (j,y)).
 
 Proposition preserve_Injectivity_implies_preserving_view_injectivity :
-  forall A B (f : ViewArray A -> ViewArray B), preserve_Injectivity f -> (forall v, Injective v -> Injective (f v)).
+  forall A B (f : CurryViewArray A -> CurryViewArray B), preserve_Injectivity f ->
+  (forall v, Injective v -> (forall x y, (f (currying v)) x = (f (currying v)) y -> x = y)).
 Proof.
   unfold preserve_Injectivity.
   intros A B f Hf v Hinj x y.
@@ -46,7 +56,7 @@ Qed.
 
 (** reverse *)
 Proposition reverse_preserves_injectivity :
-  forall T n, preserve_Injectivity reverse (A := (n::T)).
+  forall T n, preserve_Injectivity (view reverse) (A := (n::T)).
 Proof.
   intros T n C v Hinj i j x y H.
   assert (function_injective : (forall (x y : Idx n), n - 1 - to_nat x = n - 1 - to_nat y -> x = y)). {
@@ -88,7 +98,7 @@ Qed.
 
 (** take_left *)
 Proposition take_left_preserves_injectivity :
-  forall T n b, preserve_Injectivity (take_left b) (A := ((b+n)::T)).
+  forall T n b, preserve_Injectivity (view (take_left b)) (A := ((b+n)::T)).
 Proof.
   intros T n b C v Hinj i j x y H.
   assert (function_injective : (forall (x y : Idx (b)), to_nat x = to_nat y -> x = y)). {
@@ -127,7 +137,7 @@ Qed.
 
 (** take_right *)
 Proposition take_right_preserves_injectivity :
-  forall T n a, preserve_Injectivity (take_right a) (A := ((a+n)::T)).
+  forall T n a, preserve_Injectivity (view (take_right a)) (A := ((a+n)::T)).
 Proof.
   intros T n a C v Hinj i j x y H.
   assert (function_injective : (forall (x y : Idx n), a + to_nat x = a + to_nat y -> x = y)). {
@@ -167,7 +177,7 @@ Qed.
 
 (** select_range *)
 Proposition select_range_preserves_injectivity :
-  forall T n a b, preserve_Injectivity (select_range a b) (A := ((b+n)::T)).
+  forall T n a b, preserve_Injectivity (view (select_range a b)) (A := ((b+n)::T)).
 Proof.
   intros T n a b C v Hinj i j x y H.
   assert (function_injective : (forall (x y : Idx (b-a)), a + to_nat x = a + to_nat y -> x = y)). {
@@ -207,7 +217,7 @@ Qed.
 
 (** transpose *)
 Proposition transpose_preserves_injectivity :
-  forall T m n, preserve_Injectivity transpose (A := (m::n::T)).
+  forall T m n, preserve_Injectivity (view transpose) (A := (m::n::T)).
 Proof.
   unfold preserve_Injectivity.
   intros T m n C v Hinj i j x y H.
@@ -245,7 +255,7 @@ Qed.
 
 (** group *)
 Proposition group_preserves_injectivity :
-  forall T m n, preserve_Injectivity (group m) (A := (m*n::T)).
+  forall T m n, preserve_Injectivity (view (group m)) (A := (m*n::T)).
 Proof.
   unfold preserve_Injectivity.
   intros T m n C v Hinj i j x y H.
@@ -290,12 +300,12 @@ Qed.
 
 (** map *)
 Proposition map_preserves_injectivity :
-  forall A B (n : nat) (f : ViewArray A -> ViewArray B), preserve_Injectivity f -> preserve_Injectivity (map f (n := n)).
+  forall A B (n : nat) (f : CurryViewArray A -> CurryViewArray B), preserve_Injectivity f -> preserve_Injectivity (map f (n := n)).
 Proof.
   unfold preserve_Injectivity.
   intros A B n f Hf C v Hinj i j x y H.
   assert (function_injective : forall (xi yi : Idx n) (tx ty : (Tuple B)),
-      curry_totalApp (f (curry_partialApp v i xi)) tx = curry_totalApp (f (curry_partialApp v j yi)) ty ->
+      (f (currying (curry_partialApp v i xi))) tx = (f (currying (curry_partialApp v j yi))) ty ->
       ((xi,i),tx) = ((yi,j),ty)). {
     intros xi yi tx ty H'.
     assert (Hx:curry_partialApp v i xi = curry_partialApp (reorder v) (A := (n::C)) (xi,i)).
@@ -314,4 +324,17 @@ Proof.
   injection H. intros;subst;split;reflexivity.
 Qed.
 
-
+Theorem injective_functions_preserve_injectivity :
+  forall A B (f : Tuple B -> Tuple A),
+  (forall x y, f x = f y -> x = y) -> preserve_Injectivity (view f).
+Proof.
+  intros A B f Hf C v Hinj i j x y H.
+  destruct C.
+  + destruct i,j. unfold Injective in Hinj. unfold currying in *. unfold view in *. simpl in *.
+  apply Hinj in H. apply Hf in H. subst. reflexivity.
+  + destruct i as [i ti],j as [j tj]. unfold currying in *. unfold view in *. simpl in *.
+  assert (Heq : curry_totalApp (curry_partialApp v (i,ti) (A := (h::C))) (f x) = curry_totalApp (curry_partialApp v (j,tj) (A := (h::C))) (f y)
+        -> ((i,ti),f x) = ((j,tj),f y)).
+  apply injectivity_decomposition. apply Hinj. apply Heq in H.
+  inversion H. apply Hf in H3. subst. reflexivity.
+Qed.
